cedar-lean/Cedar/Thm/Partial/Evaluation/Binary.lean
@@ -92,12 +92,13 @@ theorem evaluateBinaryApp_on_concrete_eqv_concrete {op : BinaryOp} {v₁ v₂ : 
   `Spec.Expr.binaryApp` with the same subexpressions
 -/
 theorem on_concrete_eqv_concrete_eval {x₁ x₂ : Spec.Expr} {request : Spec.Request} {entities : Spec.Entities} {op : BinaryOp} :
-  Partial.evaluate x₁ request entities = (Spec.evaluate x₁ request entities).map Partial.Value.value →
-  Partial.evaluate x₂ request entities = (Spec.evaluate x₂ request entities).map Partial.Value.value →
-  Partial.evaluate (Partial.Expr.binaryApp op x₁ x₂) request entities = (Spec.evaluate (Spec.Expr.binaryApp op x₁ x₂) request entities).map Partial.Value.value
+  PartialEvalEquivConcreteEval x₁ request entities →
+  PartialEvalEquivConcreteEval x₂ request entities →
+  PartialEvalEquivConcreteEval (Spec.Expr.binaryApp op x₁ x₂) request entities
 := by
+  unfold PartialEvalEquivConcreteEval
   intro ih₁ ih₂
-  unfold Partial.evaluate Spec.evaluate
+  unfold Partial.evaluate Spec.evaluate Spec.Expr.asPartialExpr
   simp only [ih₁, ih₂, Except.map]
   cases h₁ : Spec.evaluate x₁ request entities <;> simp only [h₁, Except.bind_err, Except.bind_ok]
   case ok v₁ =>
